trying some things

Dec5.lean
@@ -2,10 +2,135 @@ import Utils
 
 namespace Dec5
 
-structure StackMachine (α : Type u) where
-  stacks : List (List α)
+-- Brief detour into defining a vector
+-- we're using the subtype notation
+abbrev Vector (α : Type u) (n : Nat) := { l : List α // l.length = n }
+
+def Vector.nil : Vector α 0 := ⟨[], rfl⟩
+def Vector.cons {α : Type u} (e : α) (v : Vector α n) : Vector α (n + 1) :=
+  ⟨e :: v.val, by simp exact v.property⟩
+def Vector.length {α : Type u} (_ : Vector α n) := n
+def Vector.nth {α : Type u} (v : Vector α n) (idx : Fin n) :=
+  let p : idx.val < v.val.length := by
+    have x := v.property
+    rw [x]
+    exact idx.isLt
+  v.val[idx.val]'p
+def Vector.set {α : Type u} (v : Vector α n) (idx : Fin n) (el : α) : Vector α n :=
+  ⟨ v.val.set idx.val el, by simp exact v.property ⟩
+def Vector.fromList {α} (l : List α) : Vector α l.length := ⟨ l,  rfl ⟩
+
+theorem take_length {α} (n : Nat) (l : List α) (H : (Nat.succ n) < l.length)
+        : List.length (List.take (Nat.succ n) l) = Nat.succ (List.length (List.take n l)) :=
+  sorry
+
+def Vector.truncateList {α} (l : List α) (nf : Fin (Nat.succ l.length)) : Vector α n :=
+  let ⟨ n, lt ⟩ := nf
+  -- let p : List.length (List.take n l) = n := by
+  --   induction l with
+  --   | nil => cases n with
+  --            | zero => simp [List.take]
+  --            | succ n' => simp [List.take]; simp [*] at *; sorry
+  --   | cons h t H => cases n with
+  --            | zero => simp [List.take]
+  --            | succ n' =>  simp [List.take]
+    -- induction n with
+    -- | zero => simp [List.take]
+    -- | succ n' H => cases l with
+    --                | nil => sorry
+    --                | cons h t => simp [List.take]
+
+    -- induction n.val
+    -- · simp [List.take]
+    -- · rw [take_length]
+    --   · simp assumption
+      -- · simp assumption
+
+  ⟨ l.take n , p ⟩
+
+notation a ":::" b => Vector.cons a b
+
+structure StackMachine (n : Nat) where
+  stacks : Vector (List Char) n
+deriving Repr
+  
+def StackMachine.empty : StackMachine 0 :=
+  StackMachine.mk $ Vector.nil
+  
+def StackMachine.addCol {n : Nat} (sm : StackMachine n) : StackMachine (n + 1) :=
+  StackMachine.mk $ sm.stacks.cons []
+  
+def StackMachine.take {n : Nat} (frm : Fin n) (sm : StackMachine n) : Option (Char × StackMachine n) :=
+  let stack := sm.stacks.nth frm
+  match stack with
+  | h :: tl => (h, StackMachine.mk $ sm.stacks.set frm tl)
+  | [] => none
+  
+def StackMachine.place {n : Nat} (to : Fin n) (c : Char) (sm : StackMachine n) : StackMachine n :=
+  let stack := sm.stacks.nth to
+  StackMachine.mk $ sm.stacks.set to (c :: stack)
+  
+-- Move `num` boxes from stack `frm` to stack `to`
+def StackMachine.move {n : Nat} (num : Nat) (frm : Fin n) (to : Fin n) (sm : StackMachine n) : StackMachine n :=
+  match num with
+  | 0 => sm
+  | n + 1 => 
+    let sm' := match sm.take frm with
+               | some (c, sm') => sm'.place to c
+               | none => sm
+    sm'.move n frm to
+    
+#eval StackMachine.empty
+      |> StackMachine.addCol
+      |> StackMachine.addCol
+      |> StackMachine.addCol
+      |> StackMachine.place 0 'Z'
+      |> StackMachine.place 0 'N'
+      |> StackMachine.place 1 'M'
+      |> StackMachine.place 1 'C'
+      |> StackMachine.place 1 'D'
+      |> StackMachine.place 2 'E'
+      |> StackMachine.move 1 1 0
+      |> StackMachine.move 3 0 2
 
 def data : String := "data/dec5.txt"
+
+-- def List.foldl_dep {β} {α : (x : β) -> γ} (f : α → β → α) : (init : α) → List β → α
+--   | a, List.nil      => a
+--   | a, List.cons b l => foldl_dep f (f a b) l
+
+def parseStartingMachine (l : List String) : Option (List (List Char)) := do
+  -- clean up the input
+  let clean := l |> List.reverse
+                 |> List.map String.data
+                 |> List.map (Utils.windows 4)
+                 |> List.map (List.filterMap (List.get? · 1))
+                 
+  pure clean
+  -- let hd <- clean.head?
+  -- let tl <- clean.tail?
+  
+  -- let uniform := tl.all (λ x => x.length = hd.length)
+  -- if uniform then
+  --   let init : (n : Nat) × StackMachine n := ⟨ 0, StackMachine.empty ⟩
+  --   let initMach := hd.foldl (λ ⟨ n, acc ⟩ _ => ⟨ n + 1, acc.addCol ⟩) init
+
+  --   let mach := tl.foldl
+  --               (λ oacc el =>
+  --                   (Utils.enum el).foldl (λ iacc (i, el) => iacc.place i el)
+  --                               oacc)
+  --               initMach.snd
+
+  --   some ⟨ initMach.fst, mach ⟩
+  -- else
+  --   none
+
+#eval do (<- Utils.lines data)
+      |> List.groupBy (λ (x y : String) =>
+           (x.startsWith "move" && y.startsWith "move") || (!x.startsWith "move" && !y.startsWith "move"))
+      |> (List.get! · 0)
+      |> parseStartingMachine
+      |> pure
 
 def run : IO Unit := do
 
