Utils.lean
@@ -12,4 +12,20 @@ def lines (path : String) : IO (List String) := do
   let lines := String.split text (· = '\n')
   pure $ lines.filter (· ≠ "")
 
+def windows (n : Nat) (l : List α) : List (List α) :=
+  l |> List.enum
+    |> List.map (λ (i, x) => (i / n, x)) 
+    |> List.groupBy (λ (i, _) (j, _) => i = j)
+    |> List.map (List.map Prod.snd)
+    
+def enum {α} (l : List α) : List (Fin l.length × α) :=
+  match l with
+  | [] => []
+  | h :: tl => (Fin.mk tl.length (by simp_arith), h) :: (enum tl).map (λ (f, a) => (Fin.succ f, a))
+
+-- match enum tl with
+-- | [] => [(Fin.mk 0 _, h)]
+-- | (f, e) :: rst => (Fin.mk (f + 1) _, h) :: (Fin.mk f _, e) :: rst
+                
+
 end Utils
